src/SDK/Serialize/HeaderV1.dfy
@@ -11,7 +11,7 @@ include "Header.dfy"
 include "EncryptionContext.dfy"
 include "EncryptedDataKeys.dfy"
 
-module HeaderV2 {
+module HeaderV1 {
   import Aws.Crypto
   import Seq
   import Header
@@ -23,25 +23,27 @@ module HeaderV2 {
   import opened UTF8
   import opened SerializeFunctions
 
-  type V2Header = h: Header.Header
-  | h.body.HeaderBodyV2?
+  type V1Header = h: Header.Header
+  | h.body.HeaderBodyV1?
   witness *
 
-  const VERSION_2: seq<uint8> := [2];
+  const VERSION_1: seq<uint8> := [0x01];
 
-  function method WriteHeaderV2(
-    header: V2Header
+  function method WriteHeaderV1(
+    header: V1Header
   ):
     (ret: seq<uint8>)
   {
     var connonicalEC := CanonicalEncryptionContext(header.body.encryptionContext);
 
-    VERSION_2
+    VERSION_1
+    + header.body.messageType.Serialize()
     + UInt16ToSeq(header.body.esdkSuiteId)
     + header.body.messageId
     + WriteAADSection(connonicalEC)
     + WriteEncryptedDataKeys(header.body.encryptedDataKeys)
-    // contentType?
+    + [header.body.contentType.Serialize()]
+    + [0x00, 0x00, 0x00, 0x00]
     + UInt32ToSeq(header.body.frameLength)
     + header.body.suiteData
   }
